new ordered ground resolution: ord_resolve_counterex_reducing proof sketch (thm 3.15) + old ordered ground resolution: renaming

Bachmair_Ganzinger/Multiset_Even_More.thy
@@ -19,10 +19,10 @@ qed
 
 subsection \<open>Multisets and lists\<close>
 
-definition list_of_multiset :: "'a multiset \<Rightarrow> 'a list" where
-  "list_of_multiset m = (SOME l. m = mset l)"
+definition list_of_mset :: "'a multiset \<Rightarrow> 'a list" where
+  "list_of_mset m = (SOME l. m = mset l)"
   
-lemma list_of_multiset_exi: "\<exists>l. m = mset l"
+lemma list_of_mset_exi: "\<exists>l. m = mset l"
 proof (induction rule: multiset_induct)
   case empty
   then show ?case by auto
@@ -33,8 +33,8 @@ next
   then show ?case by blast
 qed
 
-lemma [simp]: "mset (list_of_multiset m) = m"
-  by (metis (mono_tags, lifting) ex_mset list_of_multiset_def someI_ex)
+lemma [simp]: "mset (list_of_mset m) = m"
+  by (metis (mono_tags, lifting) ex_mset list_of_mset_def someI_ex)  
 
 theorem range_mset_map:
   assumes "\<forall>D. D \<in># Ds \<longrightarrow> D \<in> range f" 
@@ -42,11 +42,16 @@ theorem range_mset_map:
 proof -
   have "Ds \<in> range (image_mset f)" by (simp add: assms range_image_mset)
   then obtain Cs where Cs_p: "image_mset f Cs = Ds" by auto
-  define Cl where "Cl = list_of_multiset Cs"
+  define Cl where "Cl = list_of_mset Cs"
   then have "mset Cl = Cs" by auto
   then have "image_mset f (mset Cl) = Ds" using Cs_p by auto
   then have "mset (map f Cl) = Ds" by auto
   then show ?thesis by auto
 qed
+
+theorem list_of_mset_empty[simp]:
+  assumes "list_of_mset m = []"
+  shows "m = {#}"
+by (metis (full_types) assms ex_mset list_of_mset_def mset_zero_iff_right someI_ex) 
   
 end
